Update state libraries to work with update preds.

src/lib/state/DY.Lib.State.Map.fst
@@ -137,6 +137,28 @@ val has_map_session_invariant:
 let has_map_session_invariant #key_t #value_t #mt #invs mpred =
   has_local_bytes_state_predicate (mk_map_state_tag_and_pred mpred)
 
+val map_state_update_invariant:
+  {|crypto_invariants|} ->
+  #key_t:eqtype -> #value_t:Type0 -> {|map_types key_t value_t|} ->
+   map_predicate key_t value_t ->
+  local_state_update_predicate (map key_t value_t)
+let map_state_update_invariant #cinvs #key_t #value_t #mt mpred =
+  default_local_state_update_pred (map key_t value_t)
+
+val mk_map_state_tag_and_update_pred:
+  #key_t:eqtype -> #value_t:Type0 -> {|map_types key_t value_t|} ->
+  {|crypto_invariants|} -> map_predicate key_t value_t ->
+  dtuple2 string local_bytes_state_update_predicate
+let mk_map_state_tag_and_update_pred #key_t #value_t #mt #cinvs mpred =
+  mk_local_state_tag_and_update_pred (map_state_update_invariant mpred)
+
+unfold
+val has_map_state_update_invariant:
+  #key_t:eqtype -> #value_t:Type0 -> {|map_types key_t value_t|} ->
+  {|protocol_invariants|} -> map_predicate key_t value_t -> prop
+let has_map_state_update_invariant #key_t #value_t #mt #invs mpred =
+  has_local_bytes_state_update_predicate (mk_map_state_tag_and_update_pred mpred)
+
 (*** Map API ***)
 
 [@@ "opaque_to_smt"]
@@ -206,7 +228,8 @@ val initialize_map_invariant:
   Lemma
   (requires
     trace_invariant tr /\
-    has_map_session_invariant mpred
+    has_map_session_invariant mpred /\
+    has_map_state_update_invariant mpred
   )
   (ensures (
     let (_, tr_out) = initialize_map key_t value_t prin tr in
@@ -214,6 +237,7 @@ val initialize_map_invariant:
   ))
   [SMTPat (initialize_map key_t value_t prin tr);
    SMTPat (has_map_session_invariant mpred);
+   SMTPat (has_map_state_update_invariant mpred);
    SMTPat (trace_invariant tr)
   ]
 let initialize_map_invariant #invs #key_t #value_t #mt mpred prin tr =
@@ -232,7 +256,8 @@ val add_key_value_invariant:
   (requires
     mpred.pred tr prin sess_id key value /\
     trace_invariant tr /\
-    has_map_session_invariant mpred
+    has_map_session_invariant mpred /\
+    has_map_state_update_invariant mpred
   )
   (ensures (
     let (_, tr_out) = add_key_value prin sess_id key value tr in
@@ -240,6 +265,7 @@ val add_key_value_invariant:
   ))
   [SMTPat (add_key_value prin sess_id key value tr);
    SMTPat (has_map_session_invariant mpred);
+   SMTPat (has_map_state_update_invariant mpred);
    SMTPat (trace_invariant tr)
   ]
 let add_key_value_invariant #invs #key_t #value_t #mt mpred prin sess_id key value tr =
