src/lib/state/DY.Lib.State.PKI.fst
@@ -64,6 +64,14 @@ val has_pki_invariant: {|protocol_invariants|} -> prop
 let has_pki_invariant #invs =
   has_local_bytes_state_predicate pki_tag_and_invariant
 
+val pki_tag_and_state_update_pred: {|crypto_invariants|} -> dtuple2 string local_bytes_state_update_predicate
+let pki_tag_and_state_update_pred #ci = mk_map_state_tag_and_update_pred pki_pred
+
+unfold
+val has_pki_state_update_invariant: {|protocol_invariants|} -> prop
+let has_pki_state_update_invariant #invs =
+  has_local_bytes_state_update_predicate pki_tag_and_state_update_pred
+
 (*** PKI API ***)
 
 [@@ "opaque_to_smt"]
@@ -87,7 +95,8 @@ val initialize_pki_invariant:
   Lemma
   (requires
     trace_invariant tr /\
-    has_pki_invariant
+    has_pki_invariant /\
+    has_pki_state_update_invariant
   )
   (ensures (
     let (_, tr_out) = initialize_pki prin tr in
@@ -95,6 +104,7 @@ val initialize_pki_invariant:
   ))
   [SMTPat (initialize_pki prin tr);
    SMTPat (has_pki_invariant);
+   SMTPat (has_pki_state_update_invariant);
    SMTPat (trace_invariant tr)]
 let initialize_pki_invariant #invs prin tr =
   reveal_opaque (`%initialize_pki) (initialize_pki)
@@ -106,7 +116,8 @@ val install_public_key_invariant:
   (requires
     is_public_key_for tr pk pk_type who /\
     trace_invariant tr /\
-    has_pki_invariant
+    has_pki_invariant /\
+    has_pki_state_update_invariant
   )
   (ensures (
     let (_, tr_out) = install_public_key prin sess_id pk_type who pk tr in
@@ -114,6 +125,7 @@ val install_public_key_invariant:
   ))
   [SMTPat (install_public_key prin sess_id pk_type who pk tr);
    SMTPat (has_pki_invariant);
+   SMTPat (has_pki_state_update_invariant);
    SMTPat (trace_invariant tr)]
 let install_public_key_invariant #invs prin sess_id pk_type who pk tr =
   reveal_opaque (`%install_public_key) (install_public_key)
