src/lib/state/DY.Lib.State.PrivateKeys.fst
@@ -110,6 +110,14 @@ val has_private_keys_invariant: {|protocol_invariants|} -> prop
 let has_private_keys_invariant #invs =
   has_local_bytes_state_predicate private_keys_tag_and_invariant
 
+val private_keys_tag_and_state_update_pred: {|crypto_invariants|} -> dtuple2 string local_bytes_state_update_predicate
+let private_keys_tag_and_state_update_pred #ci = mk_map_state_tag_and_update_pred private_keys_pred
+
+unfold
+val has_private_keys_state_update_invariant: {|protocol_invariants|} -> prop
+let has_private_keys_state_update_invariant #invs =
+  has_local_bytes_state_update_predicate private_keys_tag_and_state_update_pred
+
 (*** Private Keys API ***)
 
 [@@ "opaque_to_smt"]
@@ -144,7 +152,8 @@ val initialize_private_keys_invariant:
   Lemma
   (requires
     trace_invariant tr /\
-    has_private_keys_invariant
+    has_private_keys_invariant /\
+    has_private_keys_state_update_invariant
   )
   (ensures (
     let (_, tr_out) = initialize_private_keys prin tr in
@@ -152,6 +161,7 @@ val initialize_private_keys_invariant:
   ))
   [SMTPat (initialize_private_keys prin tr);
    SMTPat (has_private_keys_invariant);
+   SMTPat (has_private_keys_state_update_invariant);
    SMTPat (trace_invariant tr)]
 let initialize_private_keys_invariant #invs prin tr =
   reveal_opaque (`%initialize_private_keys) (initialize_private_keys)
@@ -162,7 +172,8 @@ val generate_private_key_invariant:
   Lemma
   (requires
     trace_invariant tr /\
-    has_private_keys_invariant
+    has_private_keys_invariant /\
+    has_private_keys_state_update_invariant
   )
   (ensures (
     let (_, tr_out) = generate_private_key prin sess_id sk_type tr in
@@ -170,6 +181,7 @@ val generate_private_key_invariant:
   ))
   [SMTPat (generate_private_key prin sess_id sk_type tr);
    SMTPat (has_private_keys_invariant);
+   SMTPat (has_private_keys_state_update_invariant);
    SMTPat (trace_invariant tr)]
 let generate_private_key_invariant #invs prin sess_id sk_type tr =
   reveal_opaque (`%generate_private_key) (generate_private_key)
